wip
Signed-off-by: John Kastner <jkastner@amazon.com>

wip

Signed-off-by: John Kastner <jkastner@amazon.com>

wip

Signed-off-by: John Kastner <jkastner@amazon.com>

wip

Signed-off-by: John Kastner <jkastner@amazon.com>

wip

Signed-off-by: John Kastner <jkastner@amazon.com>

wip

Signed-off-by: John Kastner <jkastner@amazon.com>

wip

Signed-off-by: John Kastner <jkastner@amazon.com>

wip

Signed-off-by: John Kastner <jkastner@amazon.com>

wip

Signed-off-by: John Kastner <jkastner@amazon.com>

cedar-lean/Cedar/TPE/Input.lean
@@ -34,6 +34,115 @@ structure PartialEntityUID where
 def PartialEntityUID.asEntityUID (self : PartialEntityUID) : Option EntityUID :=
   self.id.map (⟨self.ty, ·⟩)
 
+inductive PartialAttribute (T : Type _) where
+  | present (val : T)
+  | unknown (ty : CedarType)
+deriving instance Repr, DecidableEq, Inhabited for PartialAttribute
+
+inductive PartialValue where
+  | prim (p : Prim)
+  | set (s : Set Value)
+  | record (m : Map Attr (PartialAttribute PartialValue))
+  | ext (x : Ext)
+deriving instance Repr, Inhabited for PartialValue
+
+mutual
+
+def decPValue (v₁ v₂ : PartialValue) : Decidable (v₁ = v₂) := by
+  cases v₁ <;> cases v₂ <;>
+  try { apply isFalse ; intro h ; injection h }
+  case prim.prim w₁ w₂ | ext.ext w₁ w₂ =>
+    exact match decEq w₁ w₂ with
+    | isTrue h => isTrue (by rw [h])
+    | isFalse _ => isFalse (by intro h; injection h; contradiction)
+  case set.set s₁ s₂ =>
+    exact match decEq s₁ s₂ with
+    | isTrue h => isTrue (by rw [h])
+    | isFalse h₁ => isFalse (by intro h₂; injection h₂; contradiction)
+  case record.record r₁ r₂ =>
+    cases r₁ ; cases r₂ ; rename_i r₁ r₂
+    exact match decProdAttrPValueList r₁ r₂ with
+    | isTrue h => isTrue (by rw [h])
+    | isFalse h₁ => isFalse (by intro h₂; simp [h₁] at h₂)
+
+def decProdAttrPValueList (avs₁ avs₂ : List (Attr × PartialAttribute PartialValue)) : Decidable (avs₁ = avs₂):=
+  match avs₁, avs₂ with
+  | [], [] => isTrue rfl
+  | _::_, [] | [], _::_ => isFalse (by intro; contradiction)
+  | (a₁, v₁) :: vs₁, (a₂, v₂) :: vs₂ =>
+    have decV : Decidable (Eq v₁ v₂) := by
+      cases v₁ <;> cases v₂
+      case present.present =>
+        simp only [PartialAttribute.present.injEq]
+        apply decPValue
+      case unknown.unknown =>
+        simp only [PartialAttribute.unknown.injEq]
+        exact decEq _ _
+      all_goals
+        simp only [reduceCtorEq]
+        exact instDecidableFalse
+    match decEq a₁ a₂, decV, decProdAttrPValueList vs₁ vs₂ with
+    | isTrue h₁, isTrue h₂, isTrue h₃ => isTrue (by rw [h₁, h₂, h₃])
+    | isFalse _, _, _ | _, isFalse _, _ | _, _, isFalse _ =>
+      isFalse (by simp; intros; first | contradiction | assumption)
+
+end
+
+
+instance : DecidableEq PartialValue := decPValue
+
+
+
+-- instance : LT PartialValue := sorry
+-- instance : DecidableLT PartialValue := sorry
+
+partial def PartialValue.asValue : PartialValue → Option Value
+  | .record as => (Value.record ∘ Map.make) <$> as.toList.mapM₂ λ kv =>
+    match kv.val.snd with
+    | .present pv => do some (kv.val.fst, ←pv.asValue)
+    | _ => none
+  | .prim p   => .some p
+  | .set es   => .some (.set es)
+  | .ext x    => .some (.ext x)
+
+def PartialValue.asEntityUID : PartialValue → Result EntityUID
+  | .prim (.entityUID uid) => .ok uid
+  | _ => .error Error.typeError
+
+def PartialValue.asSet : PartialValue → Result (Data.Set Value)
+  | .set s => .ok s
+  | _ => .error Error.typeError
+
+def PartialValue.asBool : PartialValue → Result Bool
+  | .prim (.bool b) => .ok b
+  | _ => .error Error.typeError
+
+def PartialValue.asString : PartialValue →  Result String
+  | .prim (.string s) => .ok s
+  | _ => .error Error.typeError
+
+def PartialValue.asInt : PartialValue →  Result Int64
+  | .prim (.int i) => .ok i
+  | _ => .error Error.typeError
+
+instance : Coe PartialValue (Result Bool) where
+  coe v := v.asBool
+
+instance : Coe PartialValue (Result Int64) where
+  coe v := v.asInt
+
+instance : Coe PartialValue (Result String) where
+  coe v := v.asString
+
+instance : Coe PartialValue (Result EntityUID) where
+  coe v := v.asEntityUID
+
+instance : Coe PartialValue (Result (Data.Set Value)) where
+  coe v := v.asSet
+
+abbrev PartialAttributes := Option (Map Attr (PartialAttribute PartialValue))
+abbrev PartialTags := Option (Map Tag (PartialAttribute PartialValue))
+
 structure PartialRequest where
   principal : PartialEntityUID
   action    : EntityUID
@@ -41,14 +150,13 @@ structure PartialRequest where
   -- We don't need type annotation here because the value of `context` can only
   -- be accessed via evaluating a `TypedExpr`, which allows us to obtain a
   -- (typed) `Residual`
-  context   : Option (Map Attr Value)
-
+  context   : PartialAttributes
 
 -- We don't need type annotations here following the rationale above
 structure PartialEntityData where
-  attrs     : Option (Map Attr Value)
+  attrs     : PartialAttributes
   ancestors : Option (Set EntityUID)
-  tags      : Option (Map Attr Value)
+  tags      : PartialTags
 
 abbrev MaybeEntityData := Option EntityData
 
@@ -68,14 +176,36 @@ def PartialEntities.get (es : PartialEntities) (uid : EntityUID) (f : PartialEnt
 
 def PartialEntities.ancestors (es : PartialEntities) (uid : EntityUID) : Option (Set EntityUID) := es.get uid PartialEntityData.ancestors
 
-def PartialEntities.tags (es : PartialEntities) (uid : EntityUID) : Option (Map Tag Value) := es.get uid PartialEntityData.tags
+def PartialEntities.tags (es : PartialEntities) (uid : EntityUID) : PartialTags := es.get uid PartialEntityData.tags
 
-def PartialEntities.attrs (es : PartialEntities) (uid : EntityUID) : Option (Map Tag Value) := es.get uid PartialEntityData.attrs
-
-
+def PartialEntities.attrs (es : PartialEntities) (uid : EntityUID) : PartialAttributes := es.get uid PartialEntityData.attrs
 
 def partialIsValid {α} (o : Option α) (f : α → Bool) : Bool :=
   (o.map f).getD true
+
+def requiredAttributePresent (r : Map Attr (PartialAttribute PartialValue)) (rty : Map Attr (Qualified CedarType)) (k : Attr) :=
+  match rty.find? k with
+  | .some qty => !qty.isRequired || (r.find? k|>.isSome)
+  | _ => true
+
+partial def PartialValue.instanceOfType (v : PartialValue) (ty : CedarType) (env : TypeEnv) : Bool :=
+  match v, ty with
+  | .prim (.bool b), .bool bty => instanceOfBoolType b bty
+  | .prim (.int _), .int => true
+  | .prim (.string _), .string => true
+  | .prim (.entityUID e), .entity ety => instanceOfEntityType e ety env
+  | .set s, .set ty => s.elts.attach.all (λ ⟨v, _⟩ => Value.instanceOfType v ty env)
+  | .record r, .record rty =>
+    r.toList.all (λ (k, _) => rty.contains k) &&
+    (r.toList.attach₂.all (λ ⟨(k, v), _⟩ => (match rty.find? k with
+        | .some qty =>
+          match v with
+          | .present v => instanceOfType v qty.getType env
+          | .unknown ty => ty == qty.getType
+        | _ => true))) &&
+    rty.toList.all (λ (k, _) => requiredAttributePresent r rty k)
+  | .ext x, .ext xty => instanceOfExtType x xty
+  | _, _ => false
 
 def requestIsValid (env : TypeEnv) (req : PartialRequest) : Bool :=
   (partialIsValid req.principal.asEntityUID λ principal =>
@@ -84,7 +214,7 @@ def requestIsValid (env : TypeEnv) (req : PartialRequest) : Bool :=
   (partialIsValid req.resource.asEntityUID λ resource =>
     instanceOfEntityType resource env.reqty.resource env) &&
   (partialIsValid req.context λ m =>
-    instanceOfType (.record m) (.record env.reqty.context) env)
+    PartialValue.instanceOfType (.record m) (.record env.reqty.context) env)
 
 def entitiesIsValid (env : TypeEnv) (es : PartialEntities) : Bool :=
   (es.toList.all entityIsValid) && (env.acts.toList.all instanceOfActionSchema)
@@ -99,10 +229,13 @@ where
         ancestors.all (λ ancestor =>
         entry.ancestors.contains ancestor.ty &&
         instanceOfEntityType ancestor ancestor.ty env)) &&
-      (partialIsValid attrs (instanceOfType · (.record entry.attrs) env)) &&
+      (partialIsValid attrs (λ attrs => PartialValue.instanceOfType (.record attrs)  (.record entry.attrs) env)) &&
       (partialIsValid tags λ tags =>
         match entry.tags? with
-        | .some tty => tags.values.all (instanceOfType · tty env)
+        | .some tty => tags.values.all (λ v =>
+          match v with
+          | .present v => PartialValue.instanceOfType v tty env
+          | .unknown ty => ty == tty)
         | .none     => tags == Map.empty)
     | .none       => false
   instanceOfActionSchema p :=
@@ -120,11 +253,27 @@ inductive ConcretizationError
   | entitiesDoNotMatch
   | invalidEnvironment
 
-def isValidAndConsistent (schema : Schema) (req₁ : Request) (es₁ : Entities) (req₂ : PartialRequest) (es₂ : PartialEntities) : Except ConcretizationError Unit :=
+partial def isValidAndConsistent (schema : Schema) (req₁ : Request) (es₁ : Entities) (req₂ : PartialRequest) (es₂ : PartialEntities) : Except ConcretizationError Unit :=
   match schema.environment? req₂.principal.ty req₂.resource.ty req₂.action with
   | .some env => do requestIsConsistent env; entitiesIsConsistent env; envIsWellFormed env
   | .none => .error .invalidEnvironment
 where
+  valueIsConsistent (env : TypeEnv) (v : Value) (pv : PartialValue) :=
+    match v, pv with
+    | .prim p, .prim p' => p == p'
+    | .ext x, .ext x' => x == x'
+    | .set s, .set s' => s == s'
+    | .record a, .record a' =>
+      (a'.toList.attach₂.all λ kv=>
+        match a.find? kv.val.fst, kv.val.snd with
+        | .some v, .present v' =>
+          valueIsConsistent env v v'
+        | .some v, .unknown ty => Value.instanceOfType v ty env
+        | .none, .present _ => false
+        | .none, .unknown _ => true) &&
+      (a.toList.all λ (k, _) => a'.find? k|>.isSome)
+    | _, _ => false
+
   requestIsConsistent env :=
   if !requestIsValid env req₂ || !requestMatchesEnvironment env req₁
   then
@@ -135,7 +284,7 @@ where
     if partialIsValid p₂.asEntityUID (· = p₁) &&
       a₁ = a₂ &&
       partialIsValid r₂.asEntityUID (· = r₁) &&
-      partialIsValid c₂ (· = c₁)
+      partialIsValid c₂ (λ c₂ => valueIsConsistent env (.record c₁) (.record c₂))
     then
       .ok ()
     else
@@ -145,17 +294,17 @@ where
     then
       .error .typeError
     else
-      if entitiesMatch then
+      if entitiesMatch env then
         .ok ()
       else
         .error .entitiesDoNotMatch
-  entitiesMatch :=
+  entitiesMatch env :=
       es₂.toList.all λ (a₂, e₂) => match es₁.find? a₂ with
         | .some e₁ =>
           let ⟨attrs₁, ancestors₁, tags₁⟩ := e₁
-          partialIsValid e₂.attrs (· = attrs₁) &&
+          partialIsValid e₂.attrs (λ a₂ => valueIsConsistent env (.record attrs₁) (.record a₂)) &&
           partialIsValid e₂.ancestors (· = ancestors₁) &&
-          partialIsValid e₂.tags (· = tags₁)
+          partialIsValid e₂.tags (λ t₂ => valueIsConsistent env (.record tags₁) (.record t₂))
         | .none => false
   envIsWellFormed env : Except ConcretizationError Unit :=
     if !env.validateWellFormed.isOk
@@ -163,7 +312,6 @@ where
       .error .typeError
     else
       .ok ()
-
 
 end Cedar.TPE
 
@@ -174,21 +322,39 @@ open Cedar.Spec
 open Cedar.Validation
 open Cedar.TPE
 
+partial def Value.asPartialValue : Value → PartialValue
+  | .prim p => .prim p
+  | .ext x => .ext x
+  | .set s => .set s
+  | .record as => .record ∘ Map.mk $ as.toList.attach₂.map λ kv => (kv.val.fst, .present kv.val.snd.asPartialValue)
+-- decreasing_by
+  --have : sizeOf as.kvs < sizeOf as := by
+  --  simp only [Map.sizeOf_lt_of_kvs]
+  --simp only [record.sizeOf_spec, gt_iff_lt]
+  --omega
+
+instance : Coe Bool PartialValue where
+  coe b := .prim (.bool b)
+
+instance {α : Type _} [Coe α Value] : Coe α PartialValue where
+  coe v := Value.asPartialValue v
+
 def Request.asPartialRequest (req : Request) : PartialRequest :=
   { principal := { ty := req.principal.ty, id := .some req.principal.eid }
   , action    := req.action
   , resource  := { ty := req.resource.ty, id := .some req.resource.eid }
-  , context   := req.context }
+  , context   := .some ∘ Map.mk $ req.context.toList.attach₂.map λ kv => (kv.val.fst, .present kv.val.snd.asPartialValue) }
 
 open Cedar.TPE
 
 def EntityData.asPartial (data : EntityData) : PartialEntityData :=
-  { attrs := (.some data.attrs)
+  { attrs := (.some ∘ Map.mk $ data.attrs.toList.attach₂.map λ kv => (kv.val.fst, .present kv.val.snd.asPartialValue))
   , ancestors := (.some data.ancestors)
-  , tags := (.some data.tags)}
+  , tags := (.some ∘ Map.mk $ data.tags.toList.attach₂.map λ kv => (kv.val.fst, .present kv.val.snd.asPartialValue))}
 
 def Entities.asPartial (entities: Entities) : PartialEntities :=
   entities.mapOnValues EntityData.asPartial
+
 
 
 end Cedar.Spec
